WIP

code/Yazi.CRC32Table.fst
@@ -1,6 +1,7 @@
 module Yazi.CRC32Table
 
 module B = LowStar.Buffer
+module BV = FStar.BitVector
 module Spec = Spec.CRC32
 module Seq = FStar.Seq
 module U8 = FStar.UInt8
@@ -39,27 +40,28 @@ private let poly_mask (i: U32.t{(U32.v i) < 32}) (p: U32.t{
   let i' = U32.v i in
   forall j. {:pattern UInt.nth p' j}
     (j >= i' ==> UInt.nth p' j == false) /\
-    (j < i' ==> UInt.nth p' j == Seq.index Spec.gf2_polynomial32 j)
+    (j < i' ==> UInt.nth p' j == Seq.index Spec.gf2_polynomial32 (31 - j))
 }): Tot (res: U32.t{
   let res' = U32.v res in
   let i' = U32.v i in
-  forall j. (j > i' ==> UInt.nth res' j == false) /\
-  (j <= i' ==> UInt.nth res' j == Seq.index Spec.gf2_polynomial32 j)
+  forall j. {:pattern UInt.nth res' j}
+    (j > i' ==> UInt.nth res' j == false) /\
+    (j <= i' ==> UInt.nth res' j == Seq.index Spec.gf2_polynomial32 (31 - j))
 }) =
-  if i = 5ul || i = 8ul || i = 9ul || i = 15ul || i = 19ul || i = 20ul || i = 21ul ||
-  i = 23ul || i = 24ul || i = 26ul || i = 27ul || i = 29ul || i = 30ul || i = 31ul then
+  if i = 0ul || i = 6ul || i = 9ul || i = 10ul || i = 16ul || i = 20ul || i = 21ul ||
+  i = 22ul || i = 24ul || i = 25ul || i = 27ul || i = 28ul || i = 30ul || i = 31ul then
   begin
     let open U32 in
     let one = 1ul in
     let shift = 31ul -^ i in
-    let mask = one <<^ (31ul -^ i) in
+    let mask = one <<^ shift in
     let res = p |^ mask in
     
     mask_logor_status #32 (v shift) (v mask) (v p);
     assert(forall j. {:pattern UInt.nth (UInt.logor (v p) (v mask)) j}
       j <> (32 - 1 - v shift) ==>
       UInt.nth (UInt.logor (v p) (v mask)) j == UInt.nth (v p) j);
-    assert_norm(Seq.index Spec.gf2_polynomial32 (v i) == true);
+    assert_norm(Seq.index Spec.gf2_polynomial32 (v shift) == true);
     res
   end else
     p
@@ -67,18 +69,86 @@ private let poly_mask (i: U32.t{(U32.v i) < 32}) (p: U32.t{
 let rec calc_polynomial (i: U32.t{U32.v i < 32}) (p: U32.t{
   let i' = U32.v i in
   let p' = U32.v p in
-  forall j.
+  forall j. {:pattern UInt.nth p' j}
     (j >= i' ==> UInt.nth p' j == false) /\
-    (j < i' ==> UInt.nth p' j == Seq.index Spec.gf2_polynomial32 j)
+    (j < i' ==> UInt.nth p' j == Seq.index Spec.gf2_polynomial32 (31 - j))
 }): Tot Spec.crc32_polynomial (decreases U32.v (U32.sub 32ul i)) =
   let open U32 in
   let p' = poly_mask i p in
   if i = 31ul then p' else calc_polynomial (i +^ 1ul) p'
 
 #set-options "--ifuel 64 --fuel 64"
+inline_for_extraction
 let gen_polynomial _: Tot Spec.crc32_polynomial =
   assert(forall i. UInt.nth (U32.v 0ul) i == false) by (
     let _ = forall_intro () in
     norm [simplify]);
 
   calc_polynomial 0ul 0ul
+#reset-options
+
+let poly_mod_head_zero (d: U32.t): Lemma
+  (requires UInt.nth (U32.v d) 31 == false)
+  (ensures Spec.poly_mod_correct d (U32.shift_right d 1ul)) =
+  ()
+
+let bv_one_aux (#n: nat{n > 0}) (v: BV.bv_t n): Lemma
+  (requires forall i.
+    (i < n - 1 ==> Seq.index v i == false) /\
+    (i == n - 1 ==> Seq.index v i == true))
+  (ensures UInt.from_vec v == 1) =
+  match n with
+  | 1 -> ()
+  | _ -> assert(Seq.equal (Seq.slice v 0 (n - 1)) (BV.zero_vec #(n - 1)))
+
+let logand_aux (#n: nat{n > 0}) (d: UInt.uint_t n): Lemma
+  (requires UInt.logand d 1 <> 1)
+  (ensures UInt.nth d (n - 1) == false) =
+  let res = UInt.logand d 1 in
+  uint_one_vec #n 1;
+  assert(forall i. i < n - 1 ==> UInt.nth res i == false);
+  if UInt.nth d (n - 1) then begin
+    assert(UInt.nth res (n - 1) == true);
+    bv_one_aux (UInt.to_vec res)
+  end else
+    ()
+
+let poly_xor_aux (d: U32.t) (p: Spec.crc32_polynomial): Lemma
+  (ensures forall i. {:pattern UInt.nth (U32.v (U32.logxor d p)) i}
+    UInt.nth (U32.v (U32.logxor d p)) i ==
+    Seq.index (Spec.poly_xor (UInt.to_vec (U32.v (Spec.u32_rev d)))) (31 - i)) = ()
+
+#set-options "--z3rlimit 120"
+let poly_xor_poly_mod (d: U32.t) (p: Spec.crc32_polynomial): Lemma
+  (requires UInt.nth (U32.v d) 31 == true)
+  (ensures
+    Spec.poly_mod (Spec.zero_vec_r 1 (UInt.to_vec (U32.v (Spec.u32_rev d)))) ==
+    Spec.poly_xor (UInt.to_vec (U32.v (Spec.u32_rev (U32.shift_right d 1ul))))) =
+  let open U32 in
+  let d' = UInt.to_vec (U32.v (Spec.u32_rev d)) in
+  let d'' = Spec.zero_vec_r 1 d' in
+  let d''' = UInt.to_vec (U32.v (Spec.u32_rev (d >>^ 1ul))) in
+  assert(Seq.head d'' == true);
+  assert(Seq.index d'' 32 == false);
+  assert(forall i. i < 32 ==> Seq.index d'' i == UInt.nth (v d) (31 - i));
+  assert(Seq.equal (Spec.poly_mod d'') (Spec.poly_xor #32 (Seq.tail d'')));
+  // assert(forall i. i < 31 ==> Seq.index d''' i == Seq.index d'' (i - 1));
+  admit()
+  
+let cell_xor (d: U32.t): Tot (res:U32.t{Spec.poly_mod_correct d res}) =
+  let open U32 in
+  let p = gen_polynomial () in
+  let d' = d >>^ 1ul in
+  if (d &^ 1ul) = 1ul then begin
+    assert(UInt.logand (v d) 1 == 1);
+    assert(UInt.nth (v d) 31 == true);
+    let res = d' ^^ p in
+    poly_xor_aux d' p;
+    poly_xor_poly_mod d p;
+    res
+  end else begin
+    assert(UInt.logand (v d) 1 <> 1);
+    logand_aux (v d);
+    poly_mod_head_zero d;
+    d'
+  end
