specs/Spec.CRC32.fst
@@ -83,54 +83,7 @@ let logxor_vec_assoc (#n: nat{n > 0}) (a b c: BV.bv_t n): Lemma
    SMTPat (BV.logxor_vec a (BV.logxor_vec b c))] =
   assert(Seq.equal (BV.logxor_vec (BV.logxor_vec a b) c) (BV.logxor_vec a (BV.logxor_vec b c)))
 
-unfold let zero_vec_l (#n: nat{n > 0}) (m: nat) (a: BV.bv_t n): Tot (res: BV.bv_t (n + m){
-  forall i. i < m ==> Seq.index res i == false /\
-    (i >= m /\ i < n + m ==> Seq.index res i == Seq.index a (i - m))
-}) =
-  match m with
-  | 0 -> a
-  | _ -> (BV.zero_vec #m) @| a
-
-unfold let zero_vec_r (#n: nat{n > 0}) (m: nat) (a: BV.bv_t n): Tot (res: BV.bv_t (n + m){
-  forall i. i < n ==> Seq.index res i == Seq.index a i /\ 
-    (i >= n /\ i < n + m ==> Seq.index res i == false)
-}) =
-  match m with
-  | 0 -> a
-  | _ -> a @| (BV.zero_vec #m)
-
-unfold let ones_vec_l (#n: nat{n > 0}) (m: nat) (a: BV.bv_t n): Tot (res: BV.bv_t (n + m){
-  forall i. (i < m ==> Seq.index res i == true) /\
-    (i >= m /\ i < n + m ==> Seq.index res i == Seq.index a (i - m))
-}) =
-  match m with
-  | 0 -> a
-  | _ -> (BV.ones_vec #m) @| a
-
-unfold let poly (n: nat{n >= 33}): Tot (p: BV.bv_t n{
-  Seq.head p == true
-}) =
-  zero_vec_r #33 (n - 33) gf2_polynomial
-
 #set-options "--z3rlimit 120 --z3seed 1"
-val poly_mod: #n: nat{n > 32} -> a: BV.bv_t n -> Tot (BV.bv_t 32)
-
-let rec poly_mod #n a =
-  let p = poly n in
-  let b = if Seq.head a then a -@ p else a in
-  assert(Seq.head b == false);
-  if n = 33 then (Seq.tail b) else poly_mod #(n - 1) (Seq.tail b)
-  
-unfold let poly_xor (#n: nat{n >= 32}) (a: BV.bv_t n): Tot (res: BV.bv_t n{
-  res == Seq.tail ((ones_vec_l 1 a) -@ poly (n + 1))
-}) =
-  let a' = ones_vec_l 1 a in
-  let p = poly (n + 1) in
-  let r = a -@ (Seq.tail p) in
-  let r' = a' -@ p in
-  assert(Seq.equal r (Seq.tail r'));
-  r
-
 let poly_xor_zero_suffix (#n: nat{n >= 32}) (a: BV.bv_t n) (m: nat) (l: nat): Lemma
   (ensures forall i. Seq.index (poly_xor (zero_vec_r m a)) i ==
     Seq.index (poly_xor (zero_vec_r l a)) i) = ()
