specs/Spec.CRC32.fsti
@@ -16,30 +16,79 @@ unfold let gf2_sub (#n: nat{n > 0}) (a b: BV.bv_t n) : Tot (BV.bv_t n) =
 let (-@) #n = gf2_sub #n
 
 unfold let is_rev (#n: nat{n > 0}) (a b: UInt.uint_t n) =
-  let av = UInt.to_vec a in
-  let bv = UInt.to_vec b in
-  forall i. {:pattern (Seq.index av i)}
-    Seq.index av i == Seq.index bv (n - i - 1)
+  forall i. {:pattern (UInt.nth a i)}
+    UInt.nth a i == UInt.nth b (n - i - 1)
 
 let is_rev_refl (#n: nat{n > 0}) (a b: UInt.uint_t n): Lemma
   (requires is_rev a b)
   (ensures is_rev b a)
   [SMTPat (is_rev a b)] =
-  let av = UInt.to_vec a in
-  let bv = UInt.to_vec b in
-  assert(forall i. Seq.index bv i == Seq.index av (n - i - 1))
+  assert(forall i. UInt.nth b i == UInt.nth a (n - i - 1))
 
 val u8_rev: v: U8.t -> Tot (res: U8.t{is_rev (U8.v v) (U8.v res)})
 
 val u32_rev: v: U32.t -> Tot (res: U32.t{is_rev (U32.v v) (U32.v res)})
 
 let gf2_polynomial = Seq.init #bool 33 (fun i ->
-  i = 0 || i = 6 || i = 9 || i = 10 || i = 16 || i = 20 || i = 21 || i = 22 || i = 24 ||
-  i = 25 || i = 27 || i = 28 || i = 30 || i = 31 || i = 32)
+  i = 0 || i = 1 || i = 2 || i = 4 || i = 5 || i = 7 || i = 8 || i = 10 || i = 11 ||
+  i = 12 || i = 16 || i = 22 || i = 23 || i = 26 || i = 32)
 
 let gf2_polynomial32 = Seq.tail gf2_polynomial
 
 type crc32_polynomial = res: U32.t{
   let res' = U32.v res in
-  forall j. UInt.nth res' j == Seq.index gf2_polynomial (j + 1)
+  is_rev res' (UInt.from_vec gf2_polynomial32)
 }
+
+unfold let zero_vec_l (#n: nat{n > 0}) (m: nat) (a: BV.bv_t n): Tot (res: BV.bv_t (n + m){
+  forall i.
+    i < m ==> Seq.index res i == false /\
+    (i >= m /\ i < n + m ==> Seq.index res i == Seq.index a (i - m))
+}) =
+  match m with
+  | 0 -> a
+  | _ -> Seq.append (BV.zero_vec #m) a
+
+unfold let zero_vec_r (#n: nat{n > 0}) (m: nat) (a: BV.bv_t n): Tot (res: BV.bv_t (n + m){
+  forall i.
+    i < n ==> Seq.index res i == Seq.index a i /\ 
+    (i >= n /\ i < n + m ==> Seq.index res i == false)
+}) =
+  match m with
+  | 0 -> a
+  | _ -> Seq.append a (BV.zero_vec #m)
+
+unfold let ones_vec_l (#n: nat{n > 0}) (m: nat) (a: BV.bv_t n): Tot (res: BV.bv_t (n + m){
+  forall i.
+    (i < m ==> Seq.index res i == true) /\
+    (i >= m /\ i < n + m ==> Seq.index res i == Seq.index a (i - m))
+}) =
+  match m with
+  | 0 -> a
+  | _ -> Seq.append (BV.ones_vec #m) a
+
+unfold let poly (n: nat{n >= 33}): Tot (p: BV.bv_t n{
+  Seq.head p == true
+}) =
+  zero_vec_r #33 (n - 33) gf2_polynomial
+
+unfold let poly_xor (#n: nat{n >= 32}) (a: BV.bv_t n): Tot (res: BV.bv_t n{
+  res == Seq.tail ((ones_vec_l 1 a) -@ poly (n + 1))
+}) =
+  let a' = ones_vec_l 1 a in
+  let p = poly (n + 1) in
+  let r = a -@ (Seq.tail p) in
+  let r' = a' -@ p in
+  assert(Seq.equal r (Seq.tail r'));
+  r
+
+let rec poly_mod (#n: nat{n > 32}) (a: BV.bv_t n): Tot (BV.bv_t 32) =
+  let p = poly n in
+  let b = if Seq.head a then a -@ p else a in
+  assert(Seq.head b == false);
+  if n = 33 then (Seq.tail b) else poly_mod #(n - 1) (Seq.tail b)
+
+unfold let poly_mod_correct (d res: U32.t) =
+  let d' = zero_vec_r 1 (UInt.to_vec (U32.v (u32_rev d))) in
+  forall i. {:pattern UInt.nth (U32.v res) i}
+    UInt.nth (U32.v res) i == Seq.index (poly_mod d') (31 - i)
